specs/lemmas/Spec.Blake2.Incremental.fsti
@@ -3,10 +3,7 @@ module Spec.Blake2.Incremental
 module S = FStar.Seq
 
 open Spec.Agile.Hash
-open Spec.Hash.Definitions
 open Spec.Hash.Incremental.Definitions
-open Spec.Hash.PadFinish
-open Spec.Hash.Lemmas
 open FStar.Mul
 
 val blake2_is_hash_incremental
